@prefix rdf: <http://www.w3.org/1999/02/22-rdf-syntax-ns#> .
@prefix rdfs: <http://www.w3.org/2000/01/rdf-schema#> .
@prefix sdo: <http://schema.org/> .
@prefix iisgv: <https://iisg.amsterdam/vocab/> .
@prefix rico: <https://www.ica.org/standards/RiC/ontology#> .
@prefix dcm: <http://purl.org/dc/dcmitype/> .

iisgv:nativeViewer a rdf:Property ;
        rdfs:label "nativeViewer"@en ;
        rdfs:comment "URL of the page with the item/record details in the native website"@en ;
        sdo:domainIncludes dcm:PhysicalObject, sdo:Article, sdo:AudioObject, sdo:CreativeWorkSeries, sdo:Book, sdo:DataCatalog, sdo:Dataset, sdo:ImageObject, sdo:MusicRecording, sdo:VideoObject, sdo:WebPage, rico:RecordSet;
        sdo:rangeIncludes sdo:URL .
iisgv:dateOfPublication a rdf:Property ;
        rdfs:label "dateOfPublication"@en ;
        rdfs:comment "Used for dates (as strings) to indicate the publication date of an item or object"@en ;
        sdo:domainIncludes dcm:PhysicalObject, sdo:Article, sdo:AudioObject, sdo:CreativeWorkSeries, sdo:Book, sdo:ImageObject, sdo:MusicRecording, sdo:VideoObject, sdo:WebPage;
        sdo:rangeIncludes sdo:datePublished .
iisgv:dateOfManufacture a rdf:Property ;
        rdfs:label "dateOfManufacture"@en ;
        rdfs:comment "Used for dates (as strings) to indicate the creation date of an item or object"@en ;
        sdo:domainIncludes sdo:Article, sdo:AudioObject, sdo:Book, sdo:ImageObject, sdo:MusicRecording, sdo:VideoObject;
        sdo:rangeIncludes sdo:dateCreated .